ind

theories/SLFWP.v
@@ -738,31 +738,22 @@ Module WPgenSubst.
 
 Definition Wpgen wpgen (t:trm) : formula :=
   match t with
-
   | (* [trm_val v] => *)  trm_val v =>
        wpgen_val v
-
   | (* [trm_var x] => *)  trm_var x =>
        wpgen_fail
-
   | (* [trm_fun x t1] => *)  trm_fixs bind_anon (x::nil) t1 =>
        wpgen_val (val_fun x t1)
-
   | (* [trm_fix f x t1] => *)  trm_fixs (bind_var f) (x::nil) t1 =>
        wpgen_val (val_fix f x t1)
-
   | (* [trm_if v0 t1 t2] => *)  trm_if (trm_val v0) t1 t2 =>
        wpgen_if v0 (wpgen t1) (wpgen t2)
-
   | (* [trm_seq t1 t2] => *)  trm_let bind_anon t1 t2 =>
        wpgen_seq (wpgen t1) (wpgen t2)
-
   | (* [trm_let x t1 t2] => *)  trm_let (bind_var x) t1 t2 =>
        wpgen_let (wpgen t1) (fun X => wpgen (subst x X t2))
-
   | (* [trm_app t1 t2] => *)  trm_apps t1 (t2::nil) => 
        wp t
-
   | (* other terms are outside of the sub-language that we consider,
        so let us here pretend that they are no such terms. *)
     _ => wpgen_fail
@@ -777,24 +768,37 @@ Parameter wpgen_fix : forall t,
   wpgen t = Wpgen wpgen t.
 
 (** We establish the soundness of [wpgen] by induction on [t].
-    The induction principle that we wish to use is that associated
-    with the sublanguage presented in [SLFRules], whose inductive
-    definition comes with the following induction principle.
-
-    Moreover, we tweak the induction hypothesis so that, in the case
-    of a [trm_let x t1 t2], the induction principle applies not just
-    to [t2], but to any subterm of the form [subst x v t2]. This
-    generalized induction principle is justified by the fact that
-    a substitution does not increase the size of a term (when the
-    size of all values is considered to be one unit). Again, we
-    prove this derived induction principle further in this file,
-    but the details are orthogonal to the matter of the present chapter. *)
+    The induction principle that comes with the sublanguage 
+    presented in [SLFRules] is as follows: *)
 
 Parameter trm_induct : forall (P : trm -> Prop),
   (forall v, P (trm_val v)) ->
   (forall x, P (trm_var x)) ->
   (forall x t1 , P t1 -> P (trm_fun x t1)) ->
   (forall (f:var) x t1, P t1 -> P (trm_fix f x t1)) ->
+  (forall t1, P t1 -> forall t2, P t2 -> P (trm_app t1 t2)) ->
+  (forall t1, P t1 -> forall t2, P t2 -> P (trm_seq t1 t2)) ->
+  (forall (x:var) t1, P t1 -> forall t2, P t2 -> P (trm_let x t1 t2)) ->
+  (forall v t1, P t1 -> forall t2, P t2 -> P (trm_if v t1 t2)) ->  
+  (forall t, P t).
+
+(** However, it does not quite suite our needs. Indeed, in the case
+    of a [trm_let x t1 t2], the induction principle applies to [t2],
+    but we need to invoke it on [subst x v t2].
+
+    We thus exploit a variant induction principle, justified by an
+    induction on the size of a term, for a definition of size where
+    all values and functions are considered to be of size one unit.
+
+    This induction principle is stated below. The details of its proof
+    are not essential here; they may be found in the appendix to the 
+    present chapter. *)
+
+Parameter trm_induct_subst : forall (P : trm -> Prop),
+  (forall v, P (trm_val v)) ->
+  (forall x, P (trm_var x)) ->
+  (forall x t1 , P (trm_fun x t1)) ->
+  (forall (f:var) x t1, P (trm_fix f x t1)) ->
   (forall t1, P t1 -> forall t2, P t2 -> P (trm_app t1 t2)) ->
   (forall t1, P t1 -> forall t2, P t2 -> P (trm_seq t1 t2)) ->
   (forall (x:var) t1, P t1 -> forall t2, (forall v, P (subst x v t2)) -> P (trm_let x t1 t2)) ->
@@ -810,7 +814,7 @@ Parameter trm_induct : forall (P : trm -> Prop),
 Theorem wpgen_sound : forall t,
   formula_sound_for t (wpgen t).
 Proof using.
-  intros. induction t using trm_induct; 
+  intros. induction t using trm_induct_subst;
    rewrite wpgen_fix; simpl.
   { applys wpgen_val_sound. }
   { applys wpgen_fail_sound. }
@@ -892,31 +896,22 @@ Definition wpgen_var (E:ctx) (x:var) : formula :=
 
 Fixpoint wpgen (E:ctx) (t:trm) : formula :=
  match t with
-
   | (* [trm_val v] => *)  trm_val v =>
        wpgen_val v
-
   | (* [trm_var x] => *)  trm_var x =>
        wpgen_var E x
-
   | (* [trm_fun x t1] => *)  trm_fixs bind_anon (x::nil) t1 =>
        wpgen_val (val_fun x (isubst (rem x E) t1))
-
   | (* [trm_fix f x t1] => *)  trm_fixs (bind_var f) (x::nil) t1 =>
        wpgen_val (val_fix f x (isubst (rem x (rem f E)) t1))
-
   | (* [trm_if v0 t1 t2] => *)  trm_if (trm_val v0) t1 t2 =>
        wpgen_if v0 (wpgen E t1) (wpgen E t2)
-
   | (* [trm_seq t1 t2] => *)  trm_let bind_anon t1 t2 =>
        wpgen_seq (wpgen E t1) (wpgen E t2)
-
   | (* [trm_let x t1 t2] => *)  trm_let (bind_var x) t1 t2 =>
        wpgen_let (wpgen E t1) (fun X => wpgen (Ctx.add x X E) t2)
-
   | (* [trm_app t1 t2] => *)  trm_apps t1 (t2::nil) => 
        wp (isubst E t)
-
   | (* other terms are outside of the sub-language that we consider,
        so let us here pretend that they are no such terms. *)
     _ => wpgen_fail
@@ -1417,4 +1412,131 @@ recursion
 
 
 *)
+
+
+
+(* ####################################################### *)
+(** * Appendix: non-structural induction and recursion *)
+
+
+(* ******************************************************* *)
+(** ** Size of a term *)
+
+(** Definition of the size of a term. Note that all values count for one unit,
+    even functions. *)
+
+Fixpoint size (t:trm) : nat :=
+  match t with
+  | (* [trm_val v] => *)  trm_val v =>
+       1
+  | (* [trm_var x] => *)  trm_var x =>
+       1
+  | (* [trm_fun x t1] => *)  trm_fixs bind_anon (x::nil) t1 =>
+       1
+  | (* [trm_fix f x t1] => *)  trm_fixs (bind_var f) (x::nil) t1 =>
+       1
+  | (* [trm_if v0 t1 t2] => *)  trm_if (trm_val v0) t1 t2 =>
+       1 + (size t1) + (size t2)
+  | (* [trm_seq t1 t2] => *)  trm_let bind_anon t1 t2 =>
+       1 + (size t1) + (size t2)
+  | (* [trm_let x t1 t2] => *)  trm_let (bind_var x) t1 t2 =>
+       1 + (size t1) + (size t2)
+  | (* [trm_app t1 t2] => *)  trm_apps t1 (t2::nil) => 
+       1 + (size t1) + (size t2)
+  | (* other terms are outside of the sub-language that we consider,
+       so let us here pretend that they are no such terms. *)
+    _ => 1
+  end.
+
+
+(* ******************************************************* *)
+(** ** An induction principle up to substitution *)
+
+(** We show how to prove [trm_induct_subst] used earlier to justify the
+    soundness of the non-structurally-decreasing definition of [wpgen].
+
+    We assume [trm_induct], the structural induction principle for 
+    our sublanguage, to carry out the proof. *)
+
+(** First, we show that substitution preserves the size. *)
+
+Lemma size_subst : forall x v t,
+  size (subst x v t) = size t.
+Proof using.
+  intros. induction t using trm_induct; intros; simpl; repeat case_if; auto.
+Qed.
+
+(** Second, we prove the desired induction principle by induction on
+    the size of the term. *)
+
+Section TrmInductSubst1.
+
+Hint Extern 1 (_ < _) => math.
+
+Lemma trm_induct_subst : forall (P : trm -> Prop),
+  (forall v, P (trm_val v)) ->
+  (forall x, P (trm_var x)) ->
+  (forall x t1 , P (trm_fun x t1)) ->
+  (forall (f:var) x t1,P (trm_fix f x t1)) ->
+  (forall t1, P t1 -> forall t2, P t2 -> P (trm_app t1 t2)) ->
+  (forall t1, P t1 -> forall t2, P t2 -> P (trm_seq t1 t2)) ->
+  (forall (x:var) t1, P t1 -> forall t2, (forall v, P (subst x v t2)) -> P (trm_let x t1 t2)) ->
+  (forall v t1, P t1 -> forall t2, P t2 -> P (trm_if v t1 t2)) ->  
+  (forall t, P t).
+Proof using.
+  introv M1 M2 M3 M4 M5 M6 M7 M8. 
+  (** Next line applies [applys well_founded_ind (wf_measure trm_size)] *)
+  intros t. induction_wf IH: size t. unfolds measure.
+  (** We perform a case analysis according to the grammar of our sublanguage;
+      ignore the generated induction hypotheses *)
+  destruct t using trm_induct; simpls; eauto.
+  { applys M7. { applys IH. math. } { intros v. applys IH. rewrite size_subst. math. } }
+Qed.
+
+End TrmInductSubst1.
+
+(** The general pattern for proving such induction principles with a more concise,
+    more robust proof script leverages a custom hint to treat the side conditions
+    of the form [measure size t1 t2], which are equivalent to [size t1 < size t2]. *)
+
+Section TrmInductSubst2.
+
+Hint Extern 1 (measure size _ _) => 
+  unfold measure; simpls; repeat rewrite size_subst; math.
+
+Lemma trm_induct_subst' : forall (P : trm -> Prop),
+  (forall v, P (trm_val v)) ->
+  (forall x, P (trm_var x)) ->
+  (forall x t1 , P (trm_fun x t1)) ->
+  (forall (f:var) x t1,P (trm_fix f x t1)) ->
+  (forall t1, P t1 -> forall t2, P t2 -> P (trm_app t1 t2)) ->
+  (forall t1, P t1 -> forall t2, P t2 -> P (trm_seq t1 t2)) ->
+  (forall (x:var) t1, P t1 -> forall t2, (forall v, P (subst x v t2)) -> P (trm_let x t1 t2)) ->
+  (forall v t1, P t1 -> forall t2, P t2 -> P (trm_if v t1 t2)) ->  
+  (forall t, P t).
+Proof using.
+  intros. induction_wf IH: size t.
+  destruct t using trm_induct; simpls; eauto.
+Qed.
+
+End TrmInductSubst2.
+
+
+
+(* ******************************************************* *)
+(** ** An induction principle *)
+
+
+(* ---------------------------------------------------------------------- *)
+(** Size of a term, where all values counting for one unit. *)
+
+(** Hint for induction on size. Proves subgoals of the form
+    [measure trm_size t1 t2], when [t1] and [t2] may have some
+    structure or involve substitutions. *)
+
+Ltac solve_measure_trm_size tt :=
+  unfold measure in *; simpls; repeat rewrite trm_size_subst; math.
+
+Hint Extern 1 (measure trm_size _ _) => solve_measure_trm_size tt.
+
 
